theories/Reduction.v
@@ -218,30 +218,16 @@ Module DeclarativeTypingProperties.
     now eapply typing_wk.
   Qed.
 
-  #[export, refine] Instance InferringDeclProperties : InferringProperties (ta := de) := {}.
-  Proof.
-    2-5: intros ;
-    repeat match goal with
-      | H : [_ |- _ ▹h _ ] |- _ => apply InfRedTy in H
-    end ;
-    now econstructor.
-    - intros.
-      now eapply typing_wk.
-  Qed.  
-
-  #[export, refine] Instance InferringRedDeclProperties : InferringRedProperties (ta := de) := {}.
-  Proof.
-    - intros.
-      now eapply typing_wk.
-    - intros.
-      econstructor ; tea.
-      now eapply RedConvTyC. 
-  Qed.
-
   #[export, refine] Instance TypingDeclProperties : TypingProperties (ta := de) := {}.
   Proof.
     - intros.
       now eapply typing_wk.
+    - intros.
+      now econstructor.
+    - intros.
+      now econstructor.
+    - intros.
+      now econstructor.
     - intros.
       now econstructor.
     - intros.
@@ -334,6 +320,6 @@ Module DeclarativeTypingProperties.
     now econstructor.
   Qed.
 
-  #[export] Instance DeclarativeTypingProperties : GenericTypingProperties de _ _ _ _ _ _ _ _ _ _ := {}.
+  #[export] Instance DeclarativeTypingProperties : GenericTypingProperties de _ _ _ _ _ _ _ _ := {}.
 
 End DeclarativeTypingProperties.
